---
title: Chapter3 Polynomials, Rational Expressions, and Functions – Module1 Polynomials and Operations Middle
lang: en-US
---


## 5.Focus 4
__The completing the square formula__  
::: wrap
- $\boldsymbol{a^2+b^2+c^2\pm ab \pm ac \pm bc}=\frac{1}{2}[(a\pm b)^2+(b\pm c)^2+(a\pm c)^2]$  
:::

### $\fbox{11}\:$Given that $\small a,b,c$ are the three sides of a triangle and satisfy $\small a^2+b^2+c^2=ab+ac+bc$, the triangle is:
::: wrap  
$
\begin{array}{lllll}
\textsf{(A)} \: \textsf{isosceles triangle} &
\textsf{(B)} \: \textsf{right triangle} &
\textsf{(C)} \: \textsf{equilateral triangle} & \\
\textsf{(D)} \: \textsf{isosceles right triangle} &
\textsf{(E)} \: \textsf{obtuse triangle} & \\
\end{array}
$  
:::
#### Solution
::: wrap  
$
\begin{array}{ll}
a^2+b^2+c^2=ab+ac+bc \\
a^2+b^2+c^2-ab-ac-bc=0 \\
a^2+b^2+c^2\pm ab \pm ac \pm bc=\frac{1}{2}[(a\pm b)^2+(b\pm c)^2+(a\pm c)^2] \\
(a-b)^2+(b-c)^2+(a-c)^2=0 \\
\textsf{non-negativity} \longrightarrow a=b=c \\
\end{array}
$  
:::  
#### Conclusion
- Derived Solution  
  ::: wrap
  > $\boldsymbol{(C)}$  
  > According to the Solution, get $\textsf{non-negativity} \longrightarrow a=b=c$, so choose $C$. 

  :::
- Formulas used  
  ::: wrap
  >$
  \begin{array}{ll}
  a^2+b^2+c^2\pm ab \pm ac \pm bc=\frac{1}{2}[(a\pm b)^2+(b\pm c)^2+(a\pm c)^2] & \href{/math/0%20Core%20Courses/12%20Chapter3%20polynomials-rational%20expressions-functions%20Module1%20polynomials%20and%20operations%20upper.html#_1-six-fundamental-formulas}{\textsf{completing the square formula}} \\
  \end{array}
  >$

  :::
- Conditions for identifying triangles  
  ::: wrap
  >$
  \begin{array}{ll}
  a^2+b^2=c^2 & \textsf{right triangle} \\
  a^2+b^2\lt c^2 & \textsf{obtuse triangle} \\
  a^2+b^2\gt c^2 \textsf{ (}c\text{ is longest side}\textsf{)} & \textsf{acute triangle} \\
  \end{array}
  >$

  :::
---

::: wrap  
### $\fbox{12}\:$If $\small x,y,z$ are real numbers, let $\small A=x^2-2y+\frac{\pi}{2}, B=y^2-2z+\frac{\pi}{3}, C=z^2-2x+\frac{\pi}{6}$, then among $\small A,B,C$:
:::  
::: wrap  
$
\begin{array}{lllll}
\textsf{(A)} \: \textsf{at least one is greater than zero} &
\textsf{(B)} \: \textsf{at least one is less than zero} & \\
\textsf{(C)} \: \textsf{all are greater than zero} &
\textsf{(D)} \: \textsf{all are less than zero} & \\
\textsf{(E)} \: \textsf{at least two are greater than zero} & \\
\end{array}
$  
:::
#### Solution
::: wrap  
$
\begin{array}{ll}
A+B+C=x^2-2y+y^2-2z+z^2-2x+(\frac{3\pi}{6}+\frac{2\pi}{6}+\frac{\pi}{6}) \\
x^2-2x+y^2-2y+z^2-2z+\pi \\
a^2\pm2a=(a\pm1)^2-1 \\
\underbrace{(x-1)^2+(y-1)^2+(z-1)^2}_{\ge0}+\underbrace{\pi-3}_{\ge0} \\
A+B+C\ge0 \Longrightarrow \textsf{at least one is positive} \\
\end{array}
$  
:::  
#### Conclusion
- Derived Solution  
  ::: wrap
  > $\boldsymbol{(A)}$  
  > According to the Solution, get $A+B+C\ge0 \Longrightarrow \textsf{at least one is positive}$, so choose $A$. 

  :::
- Formulas used  
  ::: wrap
  >$
  \begin{array}{ll}
  (a\pm b)^2=a^2\pm2ab+b^2 & \href{/math/0%20Core%20Courses/12%20Chapter3%20polynomials-rational%20expressions-functions%20Module1%20polynomials%20and%20operations%20upper.html#_1-six-fundamental-formulas}{\textsf{perfect square formula}} \\
  \end{array}
  >$

  :::
- Sign determination of the sum and product of three numbers (nonzero real numbers)  
  ::: wrap
  >$
  \begin{array}{ll}
  A+B+C \gt 0 \underset{❌}{\overset{✅}{\Longleftrightarrow}} \textsf{at least one is positive} \\
  A+B+C = 0 \underset{❌}{\overset{✅}{\Longleftrightarrow}} \textsf{two positive and one negative, or two negative and one positive} \\
  A+B+C \lt 0 \underset{❌}{\overset{✅}{\Longleftrightarrow}} \textsf{at least one is negative} \\
  A\cdot B\cdot C \gt 0 \underset{✅}{\overset{✅}{\Longleftrightarrow}} \textsf{all three positive, or two negative and one positive} \\
  A\cdot B\cdot C \lt 0 \underset{✅}{\overset{✅}{\Longleftrightarrow}} \textsf{all three negative, or two positive and one negative} \\
  \end{array}
  >$

  :::
---

## 6.Focus 5
__The sum and difference of cubes formula__  
- $a^3\pm b^3=(a\pm b)(a^2\mp ab+b^2)$ 


::: wrap  
### $\fbox{13}\:\small(x-2)(x+2)(x^4+4x^2+16)=\,\mathpunct{?}$.
:::  
::: wrap  
$
\begin{array}{lllll}
\textsf{(A)} \: x^4-64 &
\textsf{(B)} \: x^5-64 &
\textsf{(C)} \: x^6-64 &
\textsf{(D)} \: x^8-32 &
\textsf{(E)} \: x^6+64 & \\
\end{array}
$  
:::
#### Solution
::: wrap  
$
\begin{array}{ll}
(x-2)(x+2)(x^4+4x^2+16) \\
(x^2-2^2)(x^4+4x^2+16) \\
(x^2-4)[(x^2)^2+4x^2+4^2] \\
a^3\pm b^3=(a\pm b)(a^2\mp ab+b^2) \\
(x^2-4)[(x^2)^2+4x^2+4^2]=(x^2)^3-4^3=x^6-64 \\
\end{array}
$  
:::  
#### Conclusion
- Derived Solution  
  ::: wrap
  > $\boldsymbol{(C)}$  
  > According to the Solution, get $(x-2)(x+2)(x^4+4x^2+16)=x^6-64$, so choose $C$. 

  :::
- Formulas used  
  ::: wrap
  >$
  \begin{array}{ll}
  a^2-b^2=(a+b)(a-b) & \href{/math/0%20Core%20Courses/12%20Chapter3%20polynomials-rational%20expressions-functions%20Module1%20polynomials%20and%20operations%20upper.html#_1-six-fundamental-formulas}{\textsf{difference of squares formula}} \\
  a^3\pm b^3=(a\pm b)(a^2\mp ab+b^2) & \href{/math/0%20Core%20Courses/12%20Chapter3%20polynomials-rational%20expressions-functions%20Module1%20polynomials%20and%20operations%20upper.html#_1-six-fundamental-formulas}{\textsf{sum and difference of cubes formula}} \\
  (a^m)^n=a^{m\cdot n} & \textsf{power of a power rule} \\
  \end{array}
  >$

  :::
---

::: wrap  
### $\fbox{14}\:\small(x+1)(x-1)(x^2+x+1)(x^2-x+1)=\,\mathpunct{?}$.
:::  
::: wrap  
$
\begin{array}{lllll}
\textsf{(A)} \: x^4-1 &
\textsf{(B)} \: x^5-1 &
\textsf{(C)} \: x^6+1 &
\textsf{(D)} \: x^8-1 &
\textsf{(E)} \: x^6-1 & \\
\end{array}
$  
:::
#### Solution
::: wrap  
$
\begin{array}{ll}
(x^3+1^3)\cdot(x^3-1^3)=(x^3)^2-1=x^6-1 \\
\end{array}
$  
:::  
#### Conclusion
- Derived Solution  
  ::: wrap
  > $\boldsymbol{(E)}$  
  > According to the Solution, get $x^6-1$, so choose $E$. 

  :::
- Formulas used  
  ::: wrap
  >$
  \begin{array}{ll}
  a^3\pm b^3=(a\pm b)(a^2\mp ab+b^2) & \href{/math/0%20Core%20Courses/12%20Chapter3%20polynomials-rational%20expressions-functions%20Module1%20polynomials%20and%20operations%20upper.html#_1-six-fundamental-formulas}{\textsf{sum and difference of cubes formula}} \\
  (a^m)^n=a^{m\cdot n} & \textsf{power of a power rule} \\
  \end{array}
  >$

  :::
---

### $\fbox{15}\:$Let real numbers $\small a,b$ satisfy $\small |a-b|=2$ and $\small |a^3-b^3|=28$. Find $\small a^2+b^2$.
::: wrap  
$
\begin{array}{lllll}
\textsf{(A)} \: 30 &
\textsf{(B)} \: 22 &
\textsf{(C)} \: 15 &
\textsf{(D)} \: 13 &
\textsf{(E)} \: \frac{32}{3} & \\
\end{array}
$  
:::
#### Solution
- $\textcolor{#228B22}{\fbox{1}}\:$Solve by letting $a>b$ to remove the absolute values  
  ::: wrap  
  $
  \begin{array}{ll}
  a>b \\
  a-b=2 \\
  a^3-b^3=(a-b)(a^2+ab+b^2)=28 \\
  a^2+ab+b^2=\frac{28}{2}=14 \\
  a-b=2 \longrightarrow (a-b)^2=2^2 \\
  a^2-2ab+b^2=4 \\
  \begin{cases}
  a^2+ab+b^2=14 & ①\\
  a^2-2ab+b^2=4 & ②\\
  \end{cases} \\
  (a^2+ab+b^2)\times2+(a^2-2ab+b^2)=14\times2+4 & ①\,\times2\,+② \\
  2a^2+2ab+2b^2+a^2-2ab+b^2=3(a^2+b^2)=32 \\
  a^2+b^2=\frac{32}{3} \\
  \end{array}
  $   
  :::
- $\textcolor{#228B22}{\fbox{2}}\:$Solve by using the non-negativity of the cubic difference formula  
  ::: wrap  
  $
  \begin{array}{ll}
  |a^3-b^3|=|(a-b)(a^2+ab+b^2)|=|a-b|\cdot\underset{\textsf{non-negativity}}{|a^2+ab+b^2|}=28 \\
  a^2+ab+b^2=\frac{28}{2}=14 \\
  a-b=2 \longrightarrow (a-b)^2=2^2 \\
  a^2-2ab+b^2=4 \\
  \begin{cases}
  a^2+ab+b^2=14 & ①\\
  a^2-2ab+b^2=4 & ②\\
  \end{cases} \\
  (a^2+ab+b^2)\times2+(a^2-2ab+b^2)=14\times2+4 & ①\,\times2\,+② \\
  2a^2+2ab+2b^2+a^2-2ab+b^2=3(a^2+b^2)=32 \\
  a^2+b^2=\frac{32}{3} \\
  \end{array}
  $   
  :::
#### Conclusion
- Derived Solution  
  ::: wrap
  > $\boldsymbol{(E)}$  
  > According to the Solution, get $a^2+b^2=\frac{32}{3}$, so choose $E$. 

  :::
- Formulas used  
  ::: wrap
  >$
  \begin{array}{ll}
  a^3\pm b^3=(a\pm b)(a^2\mp ab+b^2) & \href{/math/0%20Core%20Courses/12%20Chapter3%20polynomials-rational%20expressions-functions%20Module1%20polynomials%20and%20operations%20upper.html#_1-six-fundamental-formulas}{\textsf{sum and difference of cubes formula}} \\
  (a\pm b)^2=a^2\pm2ab+b^2 & \href{/math/0%20Core%20Courses/12%20Chapter3%20polynomials-rational%20expressions-functions%20Module1%20polynomials%20and%20operations%20upper.html#_1-six-fundamental-formulas}{\textsf{perfect square formula}} \\
  \end{array}
  >$

  :::
- Derivation of the non-negativity of $a^2\mp ab+b^2$ in the sum and difference of cubes formula  
  ::: wrap
  >$
  \begin{array}{ll}
  a^2+ab+b^2=(a+\frac{b}{2})^2+\frac{3}{4}b^2 \ge 0 \\
  a^2-ab+b^2=(a-\frac{b}{2})^2+\frac{3}{4}b^2 \ge 0 \\
  \end{array}
  >$

  :::
---

## 7.Focus 6
__The cube of a sum/difference formula__  
- $(a\pm b)^3=a^3\pm3a^2b+3ab^2\pm b^3$ 

::: wrap  
### $\fbox{16}\:$Given that $\small x(1-kx)^3=a_1x+a_2x^2+a_3x^3+a_4x^4$ holds for all real numbers $\small x$. If $\small a_2=-9$, then what are the values of $\small a_1+a_2+a_3+a_4$ and $\small a_3$, respectively $\small \mathpunct{?}$.
:::  
::: wrap  
$
\begin{array}{lllll}
\textsf{(A)} \: -8,21 &
\textsf{(B)} \: -8,27 &
\textsf{(C)} \: 8,29 & \\
\textsf{(D)} \: 8,-27 &
\textsf{(E)} \: -8,-27 & \\
\end{array}
$  
:::
#### Solution
::: wrap  
$
\begin{array}{ll}
\frac{x(1-kx)^3}{x}=\frac{a_1x+a_2x^2+a_3x^3+a_4x^4}{x} & x \ne 0 \textsf{ (nonzero denominator)} \\
(1-kx)^3=a_1+a_2x+a_3x^2+a_4x^3 \\
(1-kx)^3=1-3kx+3k^2x^2-k^3x^3 \\
a_2=-3k=-9 \\
k=\frac{-9}{-3}=3 \\
a_1+a_2x+a_3x^2+a_4x^3 = a_1+a_2+a_3+a_4 & \textsf{let }x=1 \\
a_1+a_2+a_3+a_4=(1-k)^3=(1-3)^3=-8 \\
a_3=3k^2=3\cdot3^2=27 \\
\end{array}
$  
:::  
#### Conclusion
- Derived Solution  
  ::: wrap
  > $\boldsymbol{(B)}$  
  > According to the Solution, get $a_1+a_2+a_3+a_4=-8,a_3=27$, so choose $B$. 

  :::
- Formulas used  
  ::: wrap
  >$
  \begin{array}{ll}
  (a\pm b)^3=a^3\pm3a^2b+3ab^2\pm b^3 & \href{/math/0%20Core%20Courses/12%20Chapter3%20polynomials-rational%20expressions-functions%20Module1%20polynomials%20and%20operations%20upper.html#_1-six-fundamental-formulas}{\textsf{cube of a sum/difference formula}} \\
  \end{array}
  >$

  :::
- Additionally, if the problem is $a_1-a_2+a_3-a_4$  
  ::: wrap
  >$
  \begin{array}{ll}
  \frac{x(1-kx)^3}{x}=\frac{a_1x+a_2x^2+a_3x^3+a_4x^4}{x} & x \ne 0 \textsf{ (nonzero denominator)} \\
  (1-kx)^3=a_1+a_2x+a_3x^2+a_4x^3 \\
  (1-kx)^3=1-3kx+3k^2x^2-k^3x^3 \\
  a_2=-3k=-9 \\
  k=\frac{-9}{-3}=3 \\
  a_1+a_2x+a_3x^2+a_4x^3 = a_1-a_2+a_3-a_4 & \textsf{let }x=-1 \\
  a_1-a_2+a_3-a_4=(1+k)^3=(1+3)^3=64 \\
  \end{array}
  >$

  :::
---

### $\fbox{17}\:$Given nonzero real numbers $\small a,b,c$ such that $\small a+b+c=0$, find the value of $\small a^3+b^3+c^3-3abc$.
::: wrap  
$
\begin{array}{lllll}
\textsf{(A)} \: -1 &
\textsf{(B)} \: 2 &
\textsf{(C)} \: 0 &
\textsf{(D)} \: 3 &
\textsf{(E)} \: 1 & \\
\end{array}
$  
:::
#### Solution
- $\textcolor{#228B22}{\fbox{1}}\:$`Solve by using` the method of assigning specific values  
  ::: wrap  
  $
  \begin{array}{ll}
  a+b+c=0 \\
  \textsf{let }a=b=1 \quad c=-2 \\
  1^3+1^3+(-2)^3-3\cdot1\cdot1\cdot-2 \\
  1+1-8+6=0 \\
  \end{array}
  $   
  :::
- $\textcolor{#228B22}{\fbox{2}}\:$Solve by using the condition $c=-(a+b)$  
  ::: wrap  
  $
  \begin{array}{ll}
  a+b+c=0 \\
  c=-(a+b) \\
  a^3+b^3-(a+b)^3+3ab(a+b) \\
  a^3+b^3+3a^2b+3ab^2-(a+b)^3 \\
  (a+b)^3-(a+b)^3=0 \\
  \end{array}
  $   
  :::
- $\textcolor{#228B22}{\fbox{3}}\:$Solve by factoring $a^3+b^3+c^3-3abc$  
  ::: wrap  
  $
  \begin{array}{ll}
  a^3+b^3+c^3-3abc \\
  a^3+b^3=(a+b)^3-3a^2b-3ab^2 \\
  (a+b)^3+c^3-3a^2b-3ab^2-3abc \\
  (a+b)^3+c^3=(a+b+c)[(a+b)^2-(a+b)c+c^2)] \\
  -3a^2b-3ab^2-3abc=-3ab(a+b+c) \\
  (a+b+c)[(a+b)^2-(a+b)c+c^2)]-3ab(a+b+c) \\
  (a+b+c)[(a+b)^2-ac-bc+c^2-3ab] \\
  (a+b+c)(a^2+2ab+b^2-ac-bc+c^2-3ab) \\
  (a+b+c)(a^2+b^2+c^2-ab-ac-bc) \\
  a^2+b^2+c^2-ab-ac-bc=\frac{1}{2}[(a-b)^2+(b-c)^2+(a-c)^2] \ge 0 \\
  a+b+c=0 \\
  0\cdot(a^2+b^2+c^2-ab-ac-bc)=0 \\
  \end{array}
  $   
  :::
#### Conclusion
- Derived Solution  
  ::: wrap
  > $\boldsymbol{(C)}$  
  > According to the Solution, get $a^3+b^3+c^3-3abc=0$, so choose $C$. 

  :::
- Formulas used  
  ::: wrap
  >$
  \begin{array}{ll}
  (a\pm b)^3=a^3\pm3a^2b+3ab^2\pm b^3 & \href{/math/0%20Core%20Courses/12%20Chapter3%20polynomials-rational%20expressions-functions%20Module1%20polynomials%20and%20operations%20upper.html#_1-six-fundamental-formulas}{\textsf{cube of a sum/difference formula}} \\
  a^3\pm b^3=(a\pm b)(a^2\mp ab+b^2) & \href{/math/0%20Core%20Courses/12%20Chapter3%20polynomials-rational%20expressions-functions%20Module1%20polynomials%20and%20operations%20upper.html#_1-six-fundamental-formulas}{\textsf{sum and difference of cubes formula}} \\
  (a\pm b)^2=a^2\pm2ab+b^2 & \href{/math/0%20Core%20Courses/12%20Chapter3%20polynomials-rational%20expressions-functions%20Module1%20polynomials%20and%20operations%20upper.html#_1-six-fundamental-formulas}{\textsf{perfect square formula}} \\
  a^2+b^2+c^2\pm ab \pm ac \pm bc=\frac{1}{2}[(a\pm b)^2+(b\pm c)^2+(a\pm c)^2] & \href{/math/0%20Core%20Courses/12%20Chapter3%20polynomials-rational%20expressions-functions%20Module1%20polynomials%20and%20operations%20upper.html#_1-six-fundamental-formulas}{\textsf{completing the square formula}} \\
  \end{array}
  >$

  :::
- Derivation of the non-negativity of completing the square formula  
  ::: wrap
  >$
  \begin{array}{ll}
  a^2+b^2+c^2-ab-ac-bc=\frac{1}{2}[(a-b)^2+(b-c)^2+(a-c)^2] \ge 0 \\
  a^2+b^2+c^2+ab+ac+bc=\frac{1}{2}[(a+b)^2+(b+c)^2+(a+c)^2] \ge 0 \\
  \end{array}
  >$

  :::
---

| Platform    | Course                                                                                                               | Coursewares                                                       |
|-------------|----------------------------------------------------------------------------------------------------------------------|-------------------------------------------------------------------|
| YouTube     | [Watch](https://www.youtube.com/watch?v=KiCsKca0_Wc&list=PLm0MFkgiW1JgKq1kku2WxmrElFbDl7p_s)                         | [Courseware](../../public/math/Core%20Courses/pdf/Courseware.pdf) |
| Dailymotion | [Watch](https://www.dailymotion.com/video/x9glvrm?playlist=x9h6d2)                                                   |                                                                   |
| Rumble      | [Watch](https://rumble.com/v6s95ab-14-chapter3-polynomials-rational-expressions-functions-module1-polynomials-.html) |                                                                   |
