---
title: Chapter3 Polynomials, Rational Expressions, and Functions – Module1 Polynomials and Operations Lower
lang: en-US
---

| Platform    | Course                                                                                                               | Coursewares                                                       |
|-------------|----------------------------------------------------------------------------------------------------------------------|-------------------------------------------------------------------|
| YouTube     | [Watch](https://www.youtube.com/watch?v=NQJPYfmdg_Q&list=PLm0MFkgiW1JgKq1kku2WxmrElFbDl7p_s)                         | [Courseware](../../public/math/Core%20Courses/pdf/Courseware.pdf) |
| Dailymotion | [Watch](https://www.dailymotion.com/video/x9glvru?playlist=x9h6d2)                                                   |                                                                   |
| Rumble      | [Watch](https://rumble.com/v6s95bl-15-chapter3-polynomials-rational-expressions-functions-module1-polynomials-.html) |                                                                   |



## 8.Addition and subtraction of polynomials
- The addition and subtraction of polynomials are relatively simple: __just combine like terms__.

## 9.Multiplication of polynomials
- Polynomial multiplication can be done using __the distributive law__,
  meaning __each term of one polynomial__ must be __multiplied by each term of the other__,
  and then __like terms are combined__.
  For example: $(a+b)(c+d)=ac+ad+bc+bd$.

## 10.Focus 7
__The evaluating polynomials__  
- In some problems involving finding __the value of an algebraic expression__,
  the problem often does not directly __give the value of the variables__,
  and it may be __difficult to determine them__ from __the given conditions__.
  In such cases,
  one usually performs __a substitution of the whole expression to find the value of the polynomial__.

### $\fbox{18}\:$Given $\small y=ax^7+bx^5+cx^3+dx+e$, where $\small a,b,c,d,e$ are constants. When $\small x=2,y=23$; and when $\small x=-2, y=-35$. Find the value of $\small e$.
::: wrap  
$
\begin{array}{lllll}
\textsf{(A)} \: 6 &
\textsf{(B)} \: -6 &
\textsf{(C)} \: 12 &
\textsf{(D)} \: -12 &
\textsf{(E)} \: 1 & \\
\end{array}
$  
:::
#### Solution
::: wrap  
$
\begin{array}{ll}
\begin{cases}
y=a2^7+b2^5+c2^3+2d+e=23 & ① \\
y=-a2^7-b2^5-c2^3-2d+e=-35 & ② \\
\end{cases} \\
a2^7+b2^5+c2^3+2d+e-a2^7-b2^5-c2^3-2d+e=23-35 & ①\,+② \\
2e=-12 \\
e=-6 \\
\end{array}
$  
:::  
#### Conclusion
- Derived Solution  
  ::: wrap
  > $\boldsymbol{(B)}$  
  > According to the Solution, get $e=-6$, so choose $B$. 

  :::
---

## 11.Focus 8
__The equality of polynomials__  
- For two polynomials to be equal,
  __the coefficients of terms with the same degree must be equal__.
  To determine __whether two polynomials are equal__,
  one must first check __whether they have the same number of terms__.
  This __is a necessary condition__, but __not a sufficient condition__,
  for two polynomials to be equal.

### $\fbox{19}\:$Given real numbers $\small a,b,c$. If the polynomials $\small f(x)=-7x+4$ and $\small \operatorname{g}(x)=a(x-1)^2-b(x+2)+c(x^2+x-2)$ are equal, then find the value of $\small a+b+c$.
::: wrap  
$
\begin{array}{lllll}
\textsf{(A)} \: 2 &
\textsf{(B)} \: 3 &
\textsf{(C)} \: 1 &
\textsf{(D)} \: -1 &
\textsf{(E)} \: -2 & \\
\end{array}
$  
:::
#### Solution
- $\textcolor{#228B22}{\fbox{1}}\:$Solve by using term-by-term equality  
  ::: wrap  
  $
  \begin{array}{ll}
  \operatorname{g}(x)=a(x-1)^2-b(x+2)+c(x^2+x-2) \\
  a(x^2-2x+1)-b(x+2)+c(x^2+x-2) \\
  \operatorname{g}(x)=(a+c)x^2+(-2a-b+c)x+a-2b-2c \\
  f(x)=-7x+4 \\
  \begin{cases}
  a+c=0 \\
  -2a-b+c=-7 \\
  a-2b-2c=4 \\
  \end{cases} \\
  c=-a \\
  \begin{cases}
  3a+b=7 & ① \\
  3a-2b=4 & ② \\
  \end{cases} \\
  (3a+b)-(3a-2b)=7-4& ①\,-② \\
  3b=3 \\ 
  b=\frac{3}{3}=1 \\
  a+b+c=b=1 \\
  \end{array}
  $   
  :::
- $\textcolor{#228B22}{\fbox{2}}\:$Solve by using the method of assigning specific values (an identity means that for the same inputs, the outputs are always the same)  
  ::: wrap  
  $
  \begin{array}{ll}
  \textcolor{#228B22}{\scriptsize\fbox{1}}\:x=1 \\
  f(1)=\operatorname{g}(1) \\
  -7\cdot1+4=a(1-1)^2-b(1+2)+c(1^2+1-2) \\
  -3=-3b \\
  b=\frac{-3}{-3}=1 \\
  \textcolor{#228B22}{\scriptsize\fbox{2}}\:x=-2 \\
  f(-2)=\operatorname{g}(-2) \\
  -7\cdot-2+4=a(-2-1)^2-b(-2+2)+c[(-2)^2-2-2] \\
  18=9a \\
  a=\frac{18}{9}=2 \\
  \textcolor{#228B22}{\scriptsize\fbox{3}}\:x=0 \\
  f(0)=\operatorname{g}(0) \\
  -7\cdot0+4=a(0-1)^2-b(0+2)+c(0^2+0-2) \\
  4=a-2b-2c \\
  4=2-2\cdot1-2c \\
  c=\frac{4}{-2}=-2 \\
  a+b+c=2+1-2=1 \\
  \end{array}
  $   
  :::
#### Conclusion
- Derived Solution  
  ::: wrap
  > $\boldsymbol{(C)}$  
  > According to the Solution, get $a+b+c=1$, so choose $C$. 

  :::
- Formulas used  
  ::: wrap
  >$
  \begin{array}{ll}
  (a\pm b)^2=a^2\pm2ab+b^2 & \href{/math/0%20Core%20Courses/12%20Chapter3%20polynomials-rational%20expressions-functions%20Module1%20polynomials%20and%20operations%20upper.html#_1-six-fundamental-formulas}{\textsf{perfect square formula}} \\
  \end{array}
  >$

  :::
---

## 12.Focus 9
__The multiplication of polynomials__  
- When multiplying polynomials,
  __the coefficient of a specific term__ can be found using __the matching method__.


### $\fbox{20}\:$Given that in the expansion of $\small (x^2+px+8)(x^2-3x+q)$, the $\small x^2$ and $\small x^3$ terms are missing, find the value of $\small p+q$.
::: wrap  
$
\begin{array}{lllll}
\textsf{(A)} \: -3 &
\textsf{(B)} \: -2 &
\textsf{(C)} \: 2 &
\textsf{(D)} \: 3 &
\textsf{(E)} \: 4 & \\
\end{array}
$  
:::
#### Solution
- $\textcolor{#228B22}{\fbox{1}}\:$No $x^2$ and $x^3$ means that the coefficients of $x^2$ and $x^3$ are zero. By matching coefficients to solve  
  ::: wrap  
  $
  \begin{array}{ll}
  (x^2+px+8)(x^2-3x+q) \\
  qx^2-3px^2+8x^2 \\
  q-3p+8=0 & \textsf{coefficient of }x^2 \\
  -3x^3+px^3 \\
  -3+p=0 & \textsf{coefficient of }x^3 \\
  p=3 \\
  q-3\cdot3+8=0 \\
  q=1 \\
  p+q=3+1=4 \\
  \end{array}
  $   
  :::
#### Conclusion
- Derived Solution  
  ::: wrap
  > $\boldsymbol{(E)}$  
  > According to the Solution, get $p+q=4$, so choose $E$. 

  :::
---

## 13.Focus 10
__The finding coefficients of a polynomial__  
- To find __the sum of coefficients of different terms__ in a polynomial,
  one can substitute __specific values for $\boldsymbol{x}$__, commonly $\boldsymbol{1}$,$\boldsymbol{-1}$, and $\boldsymbol{0}$.

### $\fbox{21}\:$Given that $\small (2x-1)^5=a_5x^5+a_4x^4+a_3x^3+a_2x^2+a_1x+a_0$ is an identity in $\small x$, find:
#### (1) $a_0+a_1+a_2+a_3+a_4+a_5=\,\mathpunct{?}$.
::: wrap  
$
\begin{array}{lllll}
\textsf{(A)} \: -1 &
\textsf{(B)} \: 1 &
\textsf{(C)} \: 32 &
\textsf{(D)} \: -32 &
\textsf{(E)} \: 64 & \\
\end{array}
$  
:::
#### (2) $a_0-a_1+a_2-a_3+a_4-a_5=\,\mathpunct{?}$.
::: wrap  
$
\begin{array}{lllll}
\textsf{(A)} \: -1 &
\textsf{(B)} \: -243 &
\textsf{(C)} \: 1 &
\textsf{(D)} \: 243 &
\textsf{(E)} \: -240 & \\
\end{array}
$  
:::
#### (3) $a_0+a_2+a_4=\,\mathpunct{?}$.
::: wrap  
$
\begin{array}{lllll}
\textsf{(A)} \: -121 &
\textsf{(B)} \: 121 &
\textsf{(C)} \: -120 &
\textsf{(D)} \: 120 &
\textsf{(E)} \: -122 & \\
\end{array}
$  
:::
#### (4) $a_1+a_2+a_3+a_4+a_5=\,\mathpunct{?}$.
::: wrap  
$
\begin{array}{lllll}
\textsf{(A)} \: 1 &
\textsf{(B)} \: 2 &
\textsf{(C)} \: -1 &
\textsf{(D)} \: -2 &
\textsf{(E)} \: 32 & \\
\end{array}
$
:::
#### Solution
::: wrap   
$
\begin{array}{ll}
\textcolor{#228B22}{\textsf{(1)}}\; a_0+a_1+a_2+a_3+a_4+a_5=f(1) & x=1 \\
\hspace{0.7cm} f(1)=(2\cdot1-1)^5=1^5=1 \\
\textcolor{#228B22}{\textsf{(2)}}\; a_0-a_1+a_2-a_3+a_4-a_5=f(-1) & x=-1 \\
\hspace{0.7cm} f(-1)=[2(-1)-1]^5=(-3)^5=-243 \\
\textcolor{#228B22}{\textsf{(3)}}\; a_0+a_2+a_4=\frac{\textcolor{#228B22}{\textsf{(1)}}+\textcolor{#228B22}{\textsf{(2)}}}{2}  \\
\hspace{0.7cm} 2(a_0+a_2+a_4)=1-243 \\
\hspace{0.7cm} \frac{\textcolor{#228B22}{\textsf{(1)}}+\textcolor{#228B22}{\textsf{(2)}}}{2}=\frac{-242}{2}=-121 \\
\textcolor{#228B22}{\textsf{(4)}}\; a_1+a_2+a_3+a_4+a_5=\textcolor{#228B22}{\textsf{(1)}}-a_0 \\
\hspace{0.7cm} a_0=f(0) & x=0 \\
\hspace{0.7cm} f(0)=(2\cdot0-1)^5=-1^5=-1 \\
\hspace{0.7cm} \textcolor{#228B22}{\textsf{(1)}}-a_0=f(1)-f(0)=1-(-1)=2 \\
\end{array}
$  
:::
#### Conclusion
- Derived Solution  
  ::: wrap
  > $\boldsymbol{(B)}$  
  > $\boldsymbol{(B)}$  
  > $\boldsymbol{(A)}$  
  > $\boldsymbol{(B)}$  
  > According to the Solution, get $\textcolor{#228B22}{\textsf{(1)}}=1,\textcolor{#228B22}{\textsf{(2)}}=-243,\textcolor{#228B22}{\textsf{(3)}}=-121,\textcolor{#228B22}{\textsf{(4)}}=2$,
  so choose $(1)\rightarrow B,(2)\rightarrow B,(3)\rightarrow A,(4)\rightarrow B$.

  :::
---

