---
title: Chapter3 Polynomials, Rational Expressions, and Functions – Module2 Rational Expressions, Module 3 Quadratic Functions
lang: en-US
---

| Platform    | Course                                                                                                               | Coursewares                                                       |
|-------------|----------------------------------------------------------------------------------------------------------------------|-------------------------------------------------------------------|
| YouTube     | [Watch](https://www.youtube.com/watch?v=ZPNYstpg-VU&list=PLm0MFkgiW1JgKq1kku2WxmrElFbDl7p_s)                         | [Courseware](../../public/math/Core%20Courses/pdf/Courseware.pdf) |
| Dailymotion | [Watch](https://www.dailymotion.com/video/x9glvrs?playlist=x9h6d2)                                                   |                                                                   |
| Rumble      | [Watch](https://rumble.com/v6s95ex-chapter3-polynomials-rational-expressions-functions-module2-rational-expres.html) |                                                                   |


# Module 3-02 Rational Expressions and Operations

## 1.Concept of Rational Expressions
- Definition: let $A$ and $B$ be __two polynomials__.
  The division $\boldsymbol{A \div B}$ can be written in __the form $\boldsymbol{\frac{A}{B}}$__.
  If __the divisor $\boldsymbol{B}$ contains a variable__, then __the expression $\boldsymbol{\frac{A}{B}}$ is called a rational expression__.
- $\boldsymbol{\frac{2}{3x+1}}$ can be __called a rational expression__.


## 2.Properties of Rational Expressions

### $\textcolor{#1E3A5F}{\fbox{1}}\:$Description
- If both the numerator and denominator of a rational expression are __multiplied or divided by the same nonzero polynomial__,
  the value of the rational expression __remains unchanged__.
- $\boldsymbol{\frac{A}{B}=\frac{AM}{BM}, \frac{A}{B}=\frac{A \div M}{B \div M}}$ ($M\ne0$ and $M$ is a polynomial)

### $\textcolor{#1E3A5F}{\fbox{2}}\:$Applications
- Sign rule: for the signs of __the numerator__, __denominator__, and __the rational expression__ itself,
  __changing any two of them does not change the value of the expression__.
  - $\boldsymbol{\frac{-a}{-b}=\frac{a}{b}, \frac{-a}{b}=\frac{a}{-b}=-\frac{a}{b}}$
- Reduction (cancellation): removing __all common factors__ of __the numerator and denominator__ of a rational expression is __called reduction__.
- Common denominator: converting several __rational expressions with different denominators__ into __equivalent expressions with the same denominator__ is __called finding a common denominator__.

  
## 3.Operations with Rational Expressions

### $\textcolor{#1E3A5F}{\fbox{1}}\:$Addition and subtraction rules
- Same denominator: when adding or subtracting rational expressions with the same denominator,
  __add or subtract the numerators__ while __keeping the denominator unchanged__.
  - $\boldsymbol{\frac{a}{c}\pm \frac{b}{c}=\frac{a \pm b}{c}}$
- Different denominators: when the denominators are different,
  __first find a common denominator__,
  then __perform addition or subtraction__.

### $\textcolor{#1E3A5F}{\fbox{2}}\:$Multiplication rule
- To multiply rational expressions,
  multiply __the numerators together for the new numerator__,
  and multiply __the denominators together for the new denominator__.
- $\boldsymbol{\frac{a}{b}\cdot\frac{c}{d}=\frac{ac}{bd}}$

### $\textcolor{#1E3A5F}{\fbox{3}}\:$Division rule
- To divide rational expressions, multiply __the dividend by the reciprocal of the divisor__.
- $\boldsymbol{\frac{a}{b} \div \frac{c}{d}=\frac{a}{b}\cdot\frac{d}{c}=\frac{ad}{bc}}$

### $\textcolor{#1E3A5F}{\fbox{4}}\:$Exponentiation rule
- To raise a rational expression to a power,
  raise __both the numerator and denominator to that power__.
- $\boldsymbol{(\frac{a}{b})^n=\frac{a^n}{b^n}}$

### $\textcolor{#1E3A5F}{\fbox{5}}\:$Complex fractions
- Can be simplified using __the division rule__.
- Can also be simplified using __the fundamental property of rational expressions__.


## 4.Simplest Form of a Rational Expression
- A rational expression is in simplest form when __its numerator and denominator have no common factors__.
  The final form of a rational expression must be __its simplest form__,
  and simplifying a rational expression usually involves __canceling common factors (reduction)__.


## 5.Focus 1
__The simplifying and evaluating rational expressions__  
- To simplify and evaluate a rational expression,
  one can first transform it into __a polynomial expression__ to determine __the relationships among the parameters__,
  and then __substitute these values back into the rational expression__ for simplification.


### $\fbox{29}\:$If $\small a,b$ are real numbers and $\small \frac{a^2b^2}{a^4-2b^4}=1$, then $\small \frac{a^2-b^2}{19a^2+96b^2}=\,\mathpunct{?}$.
::: wrap  
$
\begin{array}{lllll}
\textsf{(A)} \: \frac{1}{114} &
\textsf{(B)} \: \frac{1}{124} &
\textsf{(C)} \: \frac{1}{130} &
\textsf{(D)} \: \frac{1}{132} &
\textsf{(E)} \: \frac{1}{134} & \\
\end{array}
$  
:::
#### Solution
::: wrap  
$
\begin{array}{ll}
a^2b^2=a^4-2b^4 \\
a^4-a^2b^2-2b^4=0 \\
(a^2+b^2)(a^2-2b^2)=0 \\
a^2+b^2=0 \lor a^2=2b^2 \\
a^2=2b^2 & a^2+b^2\ne0 \textsf{ (nonzero denominator)} \\
\textsf{let }b=1 \quad a=2 \\
\frac{2^2-1^2}{19\cdot2^2+96\cdot1^2}=\frac{2-1}{19\cdot2+96}=\frac{1}{134} \\
\end{array}
$  
:::  
#### Conclusion
- Derived Solution  
  ::: wrap
  > $\boldsymbol{(E)}$  
  > According to the Solution, get $\frac{1}{134}$, so choose $E$. 

  :::
- Formulas used  
  ::: wrap
  >$
  \begin{array}{ll}
  & \href{/math/0%20Core%20Courses/15%20Chapter3%20polynomials-rational%20expressions-functions%20Module2%20rational%20expressions%20Module3%20quadratic%20functions.html#_2-properties-of-rational-expressions}{\textsf{properties of rational expressions}} \\
  abx^2+(bp+aq)x+pq=(ax+p)(bx+q) & \href{/math/0%20Core%20Courses/14%20Chapter3%20polynomials-rational%20expressions-functions%20Module1%20polynomials%20and%20operations%20lower.html#_19-focus-12}{\textsf{cross-multiplication factorization method}} \\
  x^2=a \longrightarrow x=\pm\sqrt{a} & \textsf{definition of square root} \\
  \end{array}
  >$

  :::
---

## 5.Focus 2
__The comparing the size of rational expressions__  
- When both the numerator and denominator are __different__,
  one often __fixes either the numerator or the denominator__,
  and then compares their values. 

### $\fbox{30}\:$If $\small a>b>0$ and $\small k>0$, then which of the following inequalities can hold $\small \mathpunct{?}$.
::: wrap  
$
\begin{array}{lllll}
\textsf{(A)} \: -\frac{b}{a}<-\frac{b+k}{a+k} &
\textsf{(B)} \: \frac{a}{b}>\frac{a-k}{b-k} &
\textsf{(C)} \: -\frac{b}{a}>-\frac{b+k}{a+k} & \\
\textsf{(D)} \: \frac{a}{b}<\frac{a-k}{b-k} &
\textsf{(E)} \: \frac{a}{b}<\frac{a-2k}{b-2k} & \\
\end{array}
$  
:::
#### Solution
- $\textcolor{#228B22}{\fbox{1}}\:$Solve by using subtraction to compare the difference with $0$  
  ::: wrap   
  $
  \begin{array}{ll}
  \textsf{(A)} \:\,❌\;\\
  (-\frac{b}{a}\cdot-1) < (-\frac{b+k}{a+k}\cdot-1)  = \frac{b}{a} > \frac{b+k}{a+k} \\
  \frac{b}{a}-\frac{b+k}{a+k}=\frac{b(a+k)-a(b+k)}{a(a+k)}=\frac{k(b-a)}{a(a+k)} \\
  a>b \Longrightarrow \textsf{numerator}<0 \\
  \frac{k(b-a)}{a(a+k)} < 0 \Longrightarrow \frac{b}{a}<\frac{b+k}{a+k} \\
  (\frac{b}{a}\cdot-1)<(\frac{b+k}{a+k}\cdot-1)=-\frac{b}{a}>-\frac{b+k}{a+k} \\
  \textsf{(B)} \:\,❌\;\\
  \frac{a}{b}>\frac{a-k}{b-k} \\
  \frac{a}{b}-\frac{a-k}{b-k}=\frac{a(b-k)-b(a-k)}{b(b-k)}=\frac{k(b-a)}{b(b-k)} \\
  b>0,k>0 \Longrightarrow \textsf{denominator }\pm \\
  \textsf{denominator has multiple cases, size undetermined} \\
  \textsf{use limit method: examine sign change near }0\textsf{ to compare sizes} \\
  \textsf{let }a=2 \quad b=1 \quad k=0.999 & \boldsymbol{\gt}\textsf{set denominator}\rightarrow0 \\
  f(k)=\frac{a-k}{b-k}=\frac{2-0.999}{1-0.999}=\frac{1.001}{0.001}=1001 \\
  f(0.999) \Longrightarrow \frac{a}{b}<\frac{a-k}{b-k} \\
  \textsf{(D)} \:\,❌\;\\
  \frac{a}{b}<\frac{a-k}{b-k} \\
  \textsf{let }a=2 \quad b=1 \quad k=2 & \boldsymbol{\lt}\textsf{set numerator}=0 \\
  f(k)=\frac{a-k}{b-k}=\frac{2-2}{1-2}=\frac{0}{-1}=0 \\
  f(2) \Longrightarrow \frac{a}{b}>\frac{a-k}{b-k} \\
  \textsf{both are incorrect, leading to a deadlock with mutual holding} \\
  \textsf{(E)} \:\,❌\;\\
  \frac{a}{b}<\frac{a-2k}{b-2k} \\
  \textsf{let }a=2 \quad b=1 \quad k=1 & \boldsymbol{\lt}\textsf{set numerator}=0 \\
  f(k)=\frac{a-2k}{b-2k}=\frac{2-2\cdot1}{1-2\cdot1}=\frac{0}{-1}=0 \\
  f(1) \Longrightarrow\frac{a}{b}>\frac{a-2k}{b-2k} \\
  \end{array}
  $   
  :::
- $\textcolor{#228B22}{\fbox{2}}\:$Solve by using division to compare the ratio with $1$  
  ::: wrap   
  $
  \begin{array}{ll}
  \textsf{(A)} \:\,❌\;\\
  (-\frac{b}{a}\cdot-1) < (-\frac{b+k}{a+k}\cdot-1) = \frac{b}{a} > \frac{b+k}{a+k} \\
  \frac{\frac{b}{a}}{\frac{b+k}{a+k}}=\frac{b}{a}\cdot\frac{a+k}{b+k}=\frac{ab+bk}{ab+ak}=\frac{bk}{ak} \\
  a>b \Longrightarrow \textsf{proper fraction}<1 \\
  \frac{bk}{ak} < 1 \Longrightarrow \frac{b}{a}<\frac{b+k}{a+k} \\
  (\frac{b}{a}\cdot-1)<(\frac{b+k}{a+k}\cdot-1)=-\frac{b}{a}>-\frac{b+k}{a+k} \\
  \textsf{(B)} \:\,❌\;\\
  \frac{a}{b}>\frac{a-k}{b-k} \\
  \frac{a}{b}-\frac{a-k}{b-k}=\frac{a(b-k)-b(a-k)}{b(b-k)}=\frac{k(b-a)}{b(b-k)} \\
  b>0,k>0 \Longrightarrow \textsf{denominator }\pm \\
  \textsf{denominator has multiple cases, size undetermined} \\
  \textsf{use limit method: examine sign change near }0\textsf{ to compare sizes} \\
  \textsf{let }a=2 \quad b=1 \quad k=0.999 & \boldsymbol{\gt}\textsf{set denominator}\rightarrow0 \\
  f(k)=\frac{a-k}{b-k}=\frac{2-0.999}{1-0.999}=\frac{1.001}{0.001}=1001 \\
  f(0.999) \Longrightarrow \frac{a}{b}<\frac{a-k}{b-k} \\
  \textsf{(D)},\textsf{(E)} \cdots \\
  \end{array}
  $   
  :::
#### Conclusion
- Derived Solution  
  ::: wrap
  > $\boldsymbol{(C)}$  
  > According to the Solution, get $(\frac{b}{a}\cdot-1)<(\frac{b+k}{a+k}\cdot-1)=-\frac{b}{a}>-\frac{b+k}{a+k}$, so choose $C$. 

  :::
- Methods for comparing rational expressions  
  ::: wrap  
  > 1. __Using subtraction__$^{\textsf{positive integers only}}$: compare the difference with $0$.  
  > 2. __Using division__$^{\textsf{positive integers only}}$: compare the ratio with $1$; this method is an extension of subtraction.  
  > 3. __Using the limit method__$^{\textsf{exclude}}$: examine the sign change near a certain point to compare sizes (__only for counterexample elimination with uncertain rational inequality size__).  
  >    - Find a counterexample: if one can be found, then it is incorrect. If they reference each other and a deadlock occurs, then both are incorrect.  
  >    - Sign rule for rational inequalities:
  >$
         \begin{cases} 
         \begin{array}{ll}
         \textsf{set numerator}=0 & \boldsymbol{\lt} \\
         \textsf{set denominator}\rightarrow0 & \boldsymbol{\gt} \\
         \end{array}
         \end{cases}
  >$  
  > 4. __Using the method of assigning specific values__:
  > substitute specific values for verification (may involve letting multiple specific values again).  

  :::
- The change in size of proper and improper fractions after adding $k$  
  ::: wrap  
  >$
  \begin{array}{ll}
  \textsf{let }a,b,k\textsf{ are positive} \\
  \frac{b}{a} \lt \frac{b+k}{a+k} & a \gt b \\
  \frac{b}{a} \gt \frac{b+k}{a+k} & a \lt b \\
  \end{array}
  >$

  :::
---

## 6.Focus 3
__The rational expression as a constant__  
- For a rational expression that equals __a constant__,
  one can first substitute __a specific value__ to find __that constant__,
  and then use __the ratio theorem__ or __an identity transformation__ to determine __the parameter values__.
  Additionally, if the expression is a constant, it means __the variables can be canceled out__,
  leaving only a constant.


### $\fbox{31}\:$Given that $\small a,b$ are nonzero real numbers, for all values of $\small x$ that make $\small \frac{ax+7}{bx+11}$ well-defined, this rational expression is a constant. Then what holds $\small \mathpunct{?}$.
::: wrap  
$
\begin{array}{lllll}
\textsf{(A)} \: 7a-11b=0 &
\textsf{(B)} \: 11a-7b=0 &
\textsf{(C)} \: 7a+11b=0 & \\
\textsf{(D)} \: 11a+7b=0 &
\textsf{(E)} \: 7a-11b=1 & \\
\end{array}
$  
:::
#### Solution
- $\textcolor{#228B22}{\fbox{1}}\:$Solve by using the method of assigning specific values  
  ::: wrap  
  $
  \begin{array}{ll}
  \textsf{let }x=0 \quad x=1 \\
  f(0)=f(1) \\
  \frac{7}{11}=\frac{a+7}{b+11}=\frac{a}{b} & \textsf{proportional geometric property} \\
  7b=11a \\
  b=\frac{11}{7}a \quad a=\frac{7}{11} & \textsf{property of proportions holds} \\
  11a-7b=0 \\
  \end{array}
  $  
  :::  
- $\textcolor{#228B22}{\fbox{2}}\:$Solve by using cancelable common factors  
  ::: wrap  
  $
  \begin{array}{ll}
  \frac{ax+7}{bx+11}=\frac{a\bcancel{(x+\frac{7}{a})}}{b\bcancel{(x+\frac{11}{b})}}=\textsf{constant} \\
  x+\frac{7}{a}=x+\frac{11}{b} \\
  \frac{7}{a}=\frac{11}{b} \\
  7b=11a \\
  11a-7b=0 \\
  \end{array}
  $  
  :::
#### Conclusion
- Derived Solution  
  ::: wrap
  > $\boldsymbol{(B)}$  
  > According to the Solution, get $11a-7b=0$, so choose $B$. 

  :::
- Formulas used  
  ::: wrap
  >$
  \begin{array}{ll}
  & \href{/math/0%20Core%20Courses/15%20Chapter3%20polynomials-rational%20expressions-functions%20Module2%20rational%20expressions%20Module3%20quadratic%20functions.html#_2-properties-of-rational-expressions}{\textsf{properties of rational expressions}} \\
  \end{array}
  >$

  :::
---
